[Civl] Add type param to Loc (#1031)

Test/civl/large-samples/treiber-stack.bpl
@@ -1,16 +1,16 @@
 // RUN: %parallel-boogie -lib:base -lib:node -timeLimit:0 -vcsSplitOnEveryAssert "%s" > "%t"
 // RUN: %diff "%s.expect" "%t"
 
-type LocTreiberStack = Loc;
-type LocTreiberNode = Loc;
-type StackElem T = Node LocTreiberNode T;
-type StackMap T = Map LocTreiberNode (StackElem T);
-datatype Treiber<T> { Treiber(top: Option LocTreiberNode, {:linear} nodes: StackMap T) }
+type TaggedLocNode V = TaggedLoc (Node V) Unit;
+
+datatype Treiber<V> { Treiber(top: Option (LocNode V), {:linear} nodes: Map (LocNode V) (Node V)) }
+type LocTreiber V = Loc (Treiber V);
+type TaggedLocTreiber V = TaggedLoc (Treiber V) Unit;
 
 type X; // module type parameter
 
-var {:layer 4, 5} TreiberPool: Map Loc (Vec X);
-var {:layer 0, 4} {:linear} TreiberPoolLow: Map Loc (Treiber X);
+var {:layer 4, 5} TreiberPool: Map (LocTreiber X) (Vec X);
+var {:layer 0, 4} {:linear} TreiberPoolLow: Map (LocTreiber X) (Treiber X);
 
 /// Proof outline
 /*
@@ -26,27 +26,27 @@ Layer 4: Introduce TreiberPool and abstract TreiberPoolLow to TreiberPool
 
 /// Yield invariants
 
-function {:inline} Domain(ts: Map LocTreiberStack (Treiber X), loc_t: LocTreiberStack): Set LocTreiberNode {
+function {:inline} Domain(ts: Map (LocTreiber X) (Treiber X), loc_t: LocTreiber X): Set (LocNode X) {
   ts->val[loc_t]->nodes->dom
 }
 
 yield invariant {:layer 1} Yield();
 
-yield invariant {:layer 2} TopInStack(loc_t: LocTreiberStack);
+yield invariant {:layer 2} TopInStack(loc_t: LocTreiber X);
 invariant Map_Contains(TreiberPoolLow, loc_t);
 invariant (var loc_n := Map_At(TreiberPoolLow, loc_t)->top; loc_n is None || Set_Contains(Domain(TreiberPoolLow, loc_t), loc_n->t));
-invariant (forall loc_n: LocTreiberNode :: Set_Contains(Domain(TreiberPoolLow, loc_t), loc_n) ==>
+invariant (forall loc_n: LocNode X :: Set_Contains(Domain(TreiberPoolLow, loc_t), loc_n) ==>
               (var loc_n' := Map_At(Map_At(TreiberPoolLow, loc_t)->nodes, loc_n)->next; loc_n' is None || Set_Contains(Domain(TreiberPoolLow, loc_t), loc_n'->t)));
 
-yield invariant {:layer 2} LocInStackOrNone(loc_t: LocTreiberStack, loc_n: Option LocTreiberNode);
+yield invariant {:layer 2} LocInStackOrNone(loc_t: LocTreiber X, loc_n: Option (LocNode X));
 invariant Map_Contains(TreiberPoolLow, loc_t);
 invariant loc_n is None || Set_Contains(Domain(TreiberPoolLow, loc_t), loc_n->t);
 
-yield invariant {:layer 3} LocInStack(loc_t: LocTreiberStack, loc_n: LocTreiberNode);
+yield invariant {:layer 3} LocInStack(loc_t: LocTreiber X, loc_n: LocNode X);
 invariant Map_Contains(TreiberPoolLow, loc_t);
 invariant Set_Contains(Domain(TreiberPoolLow, loc_t), loc_n);
 
-yield invariant {:layer 4} ReachInStack(loc_t: LocTreiberStack);
+yield invariant {:layer 4} ReachInStack(loc_t: LocTreiber X);
 invariant Map_Contains(TreiberPoolLow, loc_t);
 invariant (var t := TreiberPoolLow->val[loc_t]; Between(t->nodes->val, t->top, t->top, None()));
 invariant (var t := TreiberPoolLow->val[loc_t]; IsSubset(BetweenSet(t->nodes->val, t->top, None()), Domain(TreiberPoolLow, loc_t)->val));
@@ -56,7 +56,7 @@ invariant Map_At(TreiberPool, loc_t) == Abs(Map_At(TreiberPoolLow, loc_t));
 yield invariant {:layer 4} StackDom();
 invariant TreiberPool->dom == TreiberPoolLow->dom;
 
-yield invariant {:layer 4} PushLocInStack(loc_t: LocTreiberStack, node: StackElem X, new_loc_n: LocTreiberNode, {:linear} tagged_loc: One (TaggedLoc Unit));
+yield invariant {:layer 4} PushLocInStack(loc_t: LocTreiber X, node: Node X, new_loc_n: LocNode X, {:linear} tagged_loc: One (TaggedLocNode X));
 invariant Map_Contains(TreiberPoolLow, loc_t);
 invariant Set_Contains(Domain(TreiberPoolLow, loc_t), new_loc_n);
 invariant tagged_loc->val == TaggedLoc(new_loc_n, Unit());
@@ -64,26 +64,26 @@ invariant (var t := TreiberPoolLow->val[loc_t]; Map_At(t->nodes, new_loc_n) == n
 
 /// Layered implementation
 
-atomic action {:layer 5} AtomicAlloc() returns ({:linear} tagged_loc: One (TaggedLoc Unit))
+atomic action {:layer 5} AtomicAlloc() returns ({:linear} tagged_loc: One (TaggedLocTreiber X))
 {
-  var {:linear} one_loc_t: One LocTreiberStack;
-  var {:linear} tagged_locs: Set (TaggedLoc Unit);
+  var {:linear} one_loc_t: One (LocTreiber X);
+  var {:linear} tagged_locs: Set (TaggedLocTreiber X);
 
   call one_loc_t, tagged_locs := TaggedLocSet_New(UnitSet());
   call tagged_loc := One_Get(tagged_locs, TaggedLoc(one_loc_t->val, Unit()));
   assume !Map_Contains(TreiberPool, one_loc_t->val);
   TreiberPool := Map_Update(TreiberPool, one_loc_t->val, Vec_Empty());
 }
-yield procedure {:layer 4} Alloc() returns ({:linear} tagged_loc: One (TaggedLoc Unit))
+yield procedure {:layer 4} Alloc() returns ({:linear} tagged_loc: One (TaggedLocTreiber X))
 refines AtomicAlloc;
 ensures call TopInStack(tagged_loc->val->loc);
 ensures call ReachInStack(tagged_loc->val->loc);
 preserves call StackDom();
 {
-  var {:linear} one_loc_t: One LocTreiberStack;
-  var {:linear} tagged_locs: Set (TaggedLoc Unit);
-  var top: Option LocTreiberNode;
-  var {:linear} stack: StackMap X;
+  var {:linear} one_loc_t: One (LocTreiber X);
+  var {:linear} tagged_locs: Set (TaggedLocTreiber X);
+  var top: Option (LocNode X);
+  var {:linear} stack: Map (LocNode X) (Node X);
   var {:linear} treiber: Treiber X;
 
   top := None();
@@ -96,7 +96,7 @@ preserves call StackDom();
   call {:layer 4} AbsLemma(treiber);
 }
 
-atomic action {:layer 5} AtomicPush(loc_t: LocTreiberStack, x: X) returns (success: bool)
+atomic action {:layer 5} AtomicPush(loc_t: LocTreiber X, x: X) returns (success: bool)
 {
   if (*) {
     TreiberPool := Map_Update(TreiberPool, loc_t, Vec_Append(Map_At(TreiberPool, loc_t), x));
@@ -105,15 +105,15 @@ atomic action {:layer 5} AtomicPush(loc_t: LocTreiberStack, x: X) returns (succe
     success := false;
   }
 }
-yield procedure {:layer 4} Push(loc_t: LocTreiberStack, x: X) returns (success: bool)
+yield procedure {:layer 4} Push(loc_t: LocTreiber X, x: X) returns (success: bool)
 refines AtomicPush;
 preserves call TopInStack(loc_t);
 preserves call ReachInStack(loc_t);
 preserves call StackDom();
 {
-  var loc_n: Option LocTreiberNode;
-  var new_loc_n: LocTreiberNode;
-  var {:linear} tagged_loc: One (TaggedLoc Unit);
+  var loc_n: Option (LocNode X);
+  var new_loc_n: LocNode X;
+  var {:linear} tagged_loc: One (TaggedLocNode X);
   var {:layer 4} old_treiber: Treiber X;
 
   call {:layer 4} old_treiber := Copy(TreiberPoolLow->val[loc_t]);
@@ -128,7 +128,7 @@ preserves call StackDom();
   }
 }
 
-atomic action {:layer 5} AtomicPop(loc_t: LocTreiberStack) returns (success: bool, x_opt: Option X)
+atomic action {:layer 5} AtomicPop(loc_t: LocTreiber X) returns (success: bool, x_opt: Option X)
 {
   var stack: Vec X;
 
@@ -146,7 +146,7 @@ atomic action {:layer 5} AtomicPop(loc_t: LocTreiberStack) returns (success: boo
     x_opt := None();
   }
 }
-yield procedure {:layer 4} Pop(loc_t: LocTreiberStack) returns (success: bool, x_opt: Option X)
+yield procedure {:layer 4} Pop(loc_t: LocTreiber X) returns (success: bool, x_opt: Option X)
 refines AtomicPop;
 preserves call TopInStack(loc_t);
 preserves call ReachInStack(loc_t);
@@ -160,16 +160,16 @@ preserves call StackDom();
   }
 }
 
-atomic action {:layer 4} AtomicCreateNewTopOfStack(loc_t: LocTreiberStack, x: X)
-  returns (loc_n: Option LocTreiberNode, new_loc_n: LocTreiberNode, {:linear} tagged_loc: One (TaggedLoc Unit))
+atomic action {:layer 4} AtomicCreateNewTopOfStack(loc_t: LocTreiber X, x: X)
+  returns (loc_n: Option (LocNode X), new_loc_n: LocNode X, {:linear} tagged_loc: One (TaggedLocNode X))
 asserts Map_Contains(TreiberPoolLow, loc_t);
 {
-  var {:linear} one_loc_t: One LocTreiberStack;
+  var {:linear} one_loc_t: One (LocTreiber X);
   var {:linear} treiber: Treiber X;
-  var top: Option LocTreiberNode;
-  var {:linear} stack: StackMap X;
-  var {:linear} one_loc_n: One LocTreiberNode;
-  var {:linear} tagged_locs: Set (TaggedLoc Unit);
+  var top: Option (LocNode X);
+  var {:linear} stack: Map (LocNode X) (Node X);
+  var {:linear} one_loc_n: One (LocNode X);
+  var {:linear} tagged_locs: Set (TaggedLocNode X);
   
   call one_loc_t, treiber := Map_Get(TreiberPoolLow, loc_t);
   Treiber(top, stack) := treiber;
@@ -181,14 +181,14 @@ asserts Map_Contains(TreiberPoolLow, loc_t);
   treiber := Treiber(top, stack);
   call Map_Put(TreiberPoolLow, one_loc_t, treiber);
 }
-yield procedure {:layer 3} CreateNewTopOfStack(loc_t: LocTreiberStack, x: X)
-  returns (loc_n: Option LocTreiberNode, new_loc_n: LocTreiberNode, {:linear} tagged_loc: One (TaggedLoc Unit))
+yield procedure {:layer 3} CreateNewTopOfStack(loc_t: LocTreiber X, x: X)
+  returns (loc_n: Option (LocNode X), new_loc_n: LocNode X, {:linear} tagged_loc: One (TaggedLocNode X))
 preserves call TopInStack(loc_t);
 ensures call LocInStackOrNone(loc_t, Some(new_loc_n));
 refines AtomicCreateNewTopOfStack;
 {
-  var {:linear} one_loc_n: One LocTreiberNode;
-  var {:linear} tagged_locs: Set (TaggedLoc Unit);
+  var {:linear} one_loc_n: One (LocNode X);
+  var {:linear} tagged_locs: Set (TaggedLocNode X);
 
   call loc_n := ReadTopOfStack#Push(loc_t);
   call one_loc_n, tagged_locs := TaggedLocSet_New(UnitSet());
@@ -197,13 +197,13 @@ refines AtomicCreateNewTopOfStack;
   call AllocNode#0(loc_t, one_loc_n, Node(loc_n, x));
 }
 
-atomic action {:layer 4} AtomicPopIntermediate(loc_t: LocTreiberStack) returns (success: bool, x_opt: Option X)
+atomic action {:layer 4} AtomicPopIntermediate(loc_t: LocTreiber X) returns (success: bool, x_opt: Option X)
 {
-  var {:linear} one_loc_t: One LocTreiberStack;
-  var loc_n: Option LocTreiberNode;
+  var {:linear} one_loc_t: One (LocTreiber X);
+  var loc_n: Option (LocNode X);
   var {:linear} treiber: Treiber X;
-  var top: Option LocTreiberNode;
-  var {:linear} stack: StackMap X;
+  var top: Option (LocNode X);
+  var {:linear} stack: Map (LocNode X) (Node X);
   var x: X;
 
   assert Map_Contains(TreiberPoolLow, loc_t);
@@ -226,12 +226,12 @@ atomic action {:layer 4} AtomicPopIntermediate(loc_t: LocTreiberStack) returns (
     success := false;
   }
 }
-yield procedure {:layer 3} PopIntermediate(loc_t: LocTreiberStack) returns (success: bool, x_opt: Option X)
+yield procedure {:layer 3} PopIntermediate(loc_t: LocTreiber X) returns (success: bool, x_opt: Option X)
 refines AtomicPopIntermediate;
 preserves call TopInStack(loc_t);
 {
-  var loc_n, new_loc_n: Option LocTreiberNode;
-  var node: StackElem X;
+  var loc_n, new_loc_n: Option (LocNode X);
+  var node: Node X;
   var x: X;
 
   call loc_n := ReadTopOfStack#Pop(loc_t);
@@ -252,7 +252,7 @@ preserves call TopInStack(loc_t);
   }
 }
 
-yield procedure {:layer 2} ReadTopOfStack#Push(loc_t: LocTreiberStack) returns (loc_n: Option LocTreiberNode)
+yield procedure {:layer 2} ReadTopOfStack#Push(loc_t: LocTreiber X) returns (loc_n: Option (LocNode X))
 preserves call TopInStack(loc_t);
 ensures call LocInStackOrNone(loc_t, loc_n);
 refines right action {:layer 3} _ {
@@ -263,7 +263,7 @@ refines right action {:layer 3} _ {
   call loc_n := ReadTopOfStack#0(loc_t);
 }
 
-yield procedure {:layer 2} ReadTopOfStack#Pop(loc_t: LocTreiberStack) returns (loc_n: Option LocTreiberNode)
+yield procedure {:layer 2} ReadTopOfStack#Pop(loc_t: LocTreiber X) returns (loc_n: Option (LocNode X))
 preserves call TopInStack(loc_t);
 ensures call LocInStackOrNone(loc_t, loc_n);
 refines atomic action {:layer 3} _
@@ -275,7 +275,7 @@ refines atomic action {:layer 3} _
   call loc_n := ReadTopOfStack#0(loc_t);
 }
 
-right action {:layer 2,3} AtomicLoadNode#1(loc_t: LocTreiberStack, loc_n: LocTreiberNode) returns (node: StackElem X)
+right action {:layer 2,3} AtomicLoadNode#1(loc_t: LocTreiber X, loc_n: LocNode X) returns (node: Node X)
 {
   assert Map_Contains(TreiberPoolLow, loc_t);
   assert Map_Contains(Map_At(TreiberPoolLow, loc_t)->nodes, loc_n);
@@ -284,14 +284,14 @@ right action {:layer 2,3} AtomicLoadNode#1(loc_t: LocTreiberStack, loc_n: LocTre
 
 /// Primitives
 
-atomic action {:layer 1} AtomicLoadNode#0(loc_t: LocTreiberStack, loc_n: LocTreiberNode) returns (node: StackElem X)
+atomic action {:layer 1} AtomicLoadNode#0(loc_t: LocTreiber X, loc_n: LocNode X) returns (node: Node X)
 refines AtomicLoadNode#1;
 {
-  var {:linear} one_loc_t: One LocTreiberStack;
+  var {:linear} one_loc_t: One (LocTreiber X);
   var {:linear} treiber: Treiber X;
-  var top: Option LocTreiberNode;
-  var {:linear} stack: StackMap X;
-  var {:linear} one_loc_n: One LocTreiberNode;
+  var top: Option (LocNode X);
+  var {:linear} stack: Map (LocNode X) (Node X);
+  var {:linear} one_loc_n: One (LocNode X);
 
   call one_loc_t, treiber := Map_Get(TreiberPoolLow, loc_t);
   Treiber(top, stack) := treiber;
@@ -300,13 +300,13 @@ refines AtomicLoadNode#1;
   treiber := Treiber(top, stack);
   call Map_Put(TreiberPoolLow, one_loc_t, treiber);
 }
-yield procedure {:layer 0} LoadNode#0(loc_t: LocTreiberStack, loc_n: LocTreiberNode) returns (node: StackElem X);
+yield procedure {:layer 0} LoadNode#0(loc_t: LocTreiber X, loc_n: LocNode X) returns (node: Node X);
 refines AtomicLoadNode#0;
 
-yield procedure {:layer 0} ReadTopOfStack#0(loc_t: LocTreiberStack) returns (loc_n: Option LocTreiberNode);
+yield procedure {:layer 0} ReadTopOfStack#0(loc_t: LocTreiber X) returns (loc_n: Option (LocNode X));
 refines atomic action {:layer 1,2} _
 {
-  var {:linear} one_loc_t: One LocTreiberStack;
+  var {:linear} one_loc_t: One (LocTreiber X);
   var {:linear} treiber: Treiber X;
 
   call one_loc_t, treiber := Map_Get(TreiberPoolLow, loc_t);
@@ -315,10 +315,10 @@ refines atomic action {:layer 1,2} _
 }
 
 yield procedure {:layer 0} WriteTopOfStack#0(
-  loc_t: LocTreiberStack, old_loc_n: Option LocTreiberNode, new_loc_n: Option LocTreiberNode) returns (success: bool);
+  loc_t: LocTreiber X, old_loc_n: Option (LocNode X), new_loc_n: Option (LocNode X)) returns (success: bool);
 refines atomic action {:layer 1,4} _
 {
-  var {:linear} one_loc_t: One LocTreiberStack;
+  var {:linear} one_loc_t: One (LocTreiber X);
   var {:linear} treiber: Treiber X;
 
   call one_loc_t, treiber := Map_Get(TreiberPoolLow, loc_t);
@@ -331,10 +331,10 @@ refines atomic action {:layer 1,4} _
   call Map_Put(TreiberPoolLow, one_loc_t, treiber);
 }
 
-yield procedure {:layer 0} AllocNode#0(loc_t: LocTreiberStack, {:linear_in} one_loc_n: One LocTreiberNode, node: StackElem X);
+yield procedure {:layer 0} AllocNode#0(loc_t: LocTreiber X, {:linear_in} one_loc_n: One (LocNode X), node: Node X);
 refines atomic action {:layer 1,3} _
 {
-  var {:linear} one_loc_t: One LocTreiberStack;
+  var {:linear} one_loc_t: One (LocTreiber X);
   var {:linear} treiber: Treiber X;
 
   call one_loc_t, treiber := Map_Get(TreiberPoolLow, loc_t);
@@ -342,7 +342,7 @@ refines atomic action {:layer 1,3} _
   call Map_Put(TreiberPoolLow, one_loc_t, treiber);
 }
 
-yield procedure {:layer 0} AllocTreiber#0({:linear_in} one_loc_t: One LocTreiberStack, {:linear_in} treiber: Treiber X);
+yield procedure {:layer 0} AllocTreiber#0({:linear_in} one_loc_t: One (LocTreiber X), {:linear_in} treiber: Treiber X);
 refines atomic action {:layer 1,4} _
 {
   call Map_Put(TreiberPoolLow, one_loc_t, treiber);
@@ -372,8 +372,8 @@ ensures absStack == AbsDefinition(treiber');
 free ensures absStack == Abs(treiber);
 free ensures absStack == Abs(treiber');
 {
-  var loc_n: Option LocTreiberNode;
-  var n: StackElem X;
+  var loc_n: Option (LocNode X);
+  var n: Node X;
 
   if (treiber->top == None()) {
       absStack := Vec_Empty();
