Test/civl/samples/two-queues.bpl
@@ -1,18 +1,20 @@
 // RUN: %parallel-boogie -lib:base -lib:node -vcsSplitOnEveryAssert "%s" > "%t"
 // RUN: %diff "%s.expect" "%t"
 
-datatype Queue<T> { Queue(head: Loc, tail: Loc, {:linear} nodes: Map Loc (Node Loc T)) }
+datatype Queue<V> { Queue(head: LocNode V, tail: LocNode V, {:linear} nodes: Map (LocNode V) (Node V)) }
 
-var {:linear} {:layer 0, 1} queues: Map Loc (Queue int);
-var {:linear} {:layer 0, 1} pos: One (TaggedLoc Unit);
-var {:linear} {:layer 0, 1} neg: One (TaggedLoc Unit);
+type LocQueue V = Loc (Queue V);
+
+var {:linear} {:layer 0, 1} queues: Map (LocQueue int) (Queue int);
+var {:linear} {:layer 0, 1} pos: One (TaggedLoc (Queue int) Unit);
+var {:linear} {:layer 0, 1} neg: One (TaggedLoc (Queue int) Unit);
 
 function {:inline} IsAcyclic(q: Queue int): bool
 {
     Between(q->nodes->val, Some(q->head), Some(q->tail), None())
 }
 
-function {:inline} QueueElems(q: Queue int): [Loc]bool 
+function {:inline} QueueElems(q: Queue int): [LocNode int]bool
 {
     BetweenSet(q->nodes->val, Some(q->head), Some(q->tail))
 }
@@ -20,14 +22,14 @@ function {:inline} QueueElems(q: Queue int): [Loc]bool
 yield invariant {:layer 1} PosInv();
 invariant Map_Contains(queues, pos->val->loc);
 invariant (var q := Map_At(queues, pos->val->loc); IsAcyclic(q) &&
-            (forall loc_n: Loc:: QueueElems(q)[loc_n] ==>
+            (forall loc_n: LocNode int:: QueueElems(q)[loc_n] ==>
                 Map_Contains(q->nodes, loc_n) &&
                 (loc_n == q->tail || (var node := Map_At(q->nodes, loc_n); node->val > 0))));
 
 yield invariant {:layer 1} NegInv();
 invariant Map_Contains(queues, neg->val->loc);
 invariant (var q := Map_At(queues, neg->val->loc); IsAcyclic(q) &&
-            (forall loc_n: Loc:: QueueElems(q)[loc_n] ==>
+            (forall loc_n: LocNode int:: QueueElems(q)[loc_n] ==>
                 Map_Contains(q->nodes, loc_n) &&
                 (loc_n == q->tail || (var node := Map_At(q->nodes, loc_n); node->val < 0))));
 
@@ -36,7 +38,7 @@ yield procedure {:layer 1} Producer(i: int)
 preserves call PosInv();
 preserves call NegInv();
 {
-    var loc: Loc;
+    var loc: LocQueue int;
 
     assert {:layer 1} pos->val->loc != neg->val->loc;
     if (i == 0) {
@@ -53,7 +55,7 @@ preserves call NegInv();
 yield procedure {:layer 1} PosConsumer()
 preserves call PosInv();
 {
-    var loc: Loc;
+    var loc: LocQueue int;
     var i: int;
 
     call loc := ReadPos();
@@ -64,7 +66,7 @@ preserves call PosInv();
 yield procedure {:layer 1} NegConsumer()
 preserves call NegInv();
 {
-    var loc: Loc;
+    var loc: LocQueue int;
     var i: int;
 
     call loc := ReadNeg();
@@ -74,25 +76,25 @@ preserves call NegInv();
 
 // Primitives
 
-yield procedure {:layer 0} ReadPos() returns (loc: Loc);
+yield procedure {:layer 0} ReadPos() returns (loc: LocQueue int);
 refines both action {:layer 1} _ {
     loc := pos->val->loc;
 }
 
-yield procedure {:layer 0} ReadNeg() returns (loc: Loc);
+yield procedure {:layer 0} ReadNeg() returns (loc: LocQueue int);
 refines both action {:layer 1} _ {
     loc := neg->val->loc;
 }
 
-yield procedure {:layer 0} Enqueue(loc_q: Loc, i: int);
+yield procedure {:layer 0} Enqueue(loc_q: LocQueue int, i: int);
 refines action {:layer 1} _
 {
-    var {:linear} one_loc_q: One Loc;
+    var {:linear} one_loc_q: One (LocQueue int);
     var {:linear} queue: Queue int;
-    var head, tail: Loc;
-    var {:linear} nodes: Map Loc (Node Loc int);
-    var {:linear} one_loc_n, new_one_loc_n: One Loc;
-    var node: Node Loc int;
+    var head, tail: LocNode int;
+    var {:linear} nodes: Map (LocNode int) (Node int);
+    var {:linear} one_loc_n, new_one_loc_n: One (LocNode int);
+    var node: Node int;
 
     call one_loc_q, queue := Map_Get(queues, loc_q);
     Queue(head, tail, nodes) := queue;
@@ -108,16 +110,16 @@ refines action {:layer 1} _
     call Map_Put(queues, one_loc_q, queue);
 }
 
-yield procedure {:layer 0} Dequeue(loc_q: Loc) returns (i: int);
+yield procedure {:layer 0} Dequeue(loc_q: LocQueue int) returns (i: int);
 refines action {:layer 1} _
 {
-    var {:linear} one_loc_q: One Loc;
+    var {:linear} one_loc_q: One (LocQueue int);
     var {:linear} queue: Queue int;
-    var head, tail: Loc;
-    var {:linear} nodes: Map Loc (Node Loc int);
-    var {:linear} one_loc_n: One Loc;
-    var node: Node Loc int;
-    var next: Option Loc;
+    var head, tail: LocNode int;
+    var {:linear} nodes: Map (LocNode int) (Node int);
+    var {:linear} one_loc_n: One (LocNode int);
+    var node: Node int;
+    var next: Option (LocNode int);
 
     call one_loc_q, queue := Map_Get(queues, loc_q);
     Queue(head, tail, nodes) := queue;
